src/Examples/MailServer/MailHeap.v
@@ -1,0 +1,163 @@
+From iris.algebra Require Import auth gmap list.
+Require Export CSL.Refinement CSL.NamedDestruct CSL.BigDynOp.
+From RecoveryRefinement.Examples.MailServer Require Import MailAPI MailAPILemmas.
+From RecoveryRefinement.Goose.Examples Require Import MailServer.
+From RecoveryRefinement.Goose.Proof Require Import Interp.
+Require Import Goose.Proof.RefinementAdequacy.
+From RecoveryRefinement Require AtomicPair.Helpers.
+From RecoveryRefinement.Goose Require Import Machine GoZeroValues Heap GoLayer.
+From RecoveryRefinement.Goose Require Import Machine.
+From RecoveryRefinement.Goose Require Import GoZeroValues.
+
+Unset Implicit Arguments.
+
+
+
+Set Default Proof Using "Type".
+Section refinement_heap_triples.
+
+Context `{@gooseG gmodel gmodelHwf Σ, !@cfgG (Mail.Op) (Mail.l) Σ}.
+
+Import Filesys.FS.
+Import GoLayer.Go.
+Import Mail.
+
+  (* Every pointer in the abstract state should have a matching
+     pointer with the same value in the concrete state. *)
+  Definition HeapInv (σ : Mail.State) : iProp Σ :=
+    big_opDM bi_sep
+     (λ T p v,
+     match (fst v), T with
+     | ReadLocked n, (Ptr.Heap _) =>
+       Count_Typed_Heap.mapsto (hG := go_heap_inG) p (S n) Unlocked (snd v)
+     | _, _ => Count_Typed_Heap.mapsto (hG := go_heap_inG) p O (fst v) (snd v)
+     end ∗ ⌜ p ≠ gmodel.(@nullptr) _⌝)%I (Data.allocs σ.(heap)).
+
+  Global Instance HeapInv_Timeless σ:
+    Timeless (HeapInv σ).
+  Proof.
+    apply big_sepDM_timeless; first apply _.
+    intros [] ? ([]&?); apply _.
+  Qed.
+
+  Lemma HeapInv_agree_slice {T} σ sli alloc alloc' (vs vs': List.list T) status q:
+    Data.getAlloc sli.(slice.ptr) σ.(heap) = Some (status, alloc') →
+    Data.getSliceModel sli alloc' = Some vs' →
+    sli ↦{q} (alloc, vs) -∗ HeapInv σ -∗ ⌜ alloc = alloc' ∧ vs = vs' ⌝.
+  Proof.
+    iIntros (??) "Hsli Hheap".
+    rewrite /HeapInv.
+    iDestruct (big_sepDM_lookup (dec := sigPtr_eq_dec) with "Hheap") as "(Hlookup&%)".
+    { eauto. }
+    iAssert (∃ s q, Count_Typed_Heap.mapsto sli.(slice.ptr) s q alloc')%I
+      with "[Hlookup]" as (??) "Hlookup".
+    { destruct status; eauto. }
+    iDestruct "Hsli" as (??) "Hsli".
+    iDestruct (Count_Typed_Heap.mapsto_agree_generic with "[Hsli] Hlookup") as %Heq.
+    { eauto. }
+    subst. iPureIntro; split; auto. simpl in *. congruence.
+  Qed.
+
+  Lemma HeapInv_non_alloc_inv {A} σ p q (ls: List.list A):
+    q >= 0 →
+    HeapInv σ -∗ p ↦{q} ls -∗
+            ⌜ Data.getAlloc p σ.(heap) = None /\ p ≠ nullptr _ ⌝.
+  Proof.
+    iIntros (?) "Hheap Hp".
+    iDestruct "Hp" as "(%&Hp)". iSplit; last auto.
+    destruct (Data.getAlloc p σ.(heap)) as [v|] eqn:Heq_get; last by done.
+    iExFalso.
+    rewrite /HeapInv.
+    rewrite /Data.getAlloc in Heq_get.
+    iPoseProof (big_sepDM_lookup (T:=(Ptr.Heap A))
+                                 (dec := sigPtr_eq_dec) with "Hheap") as "(Hheap&%)"; eauto.
+    destruct v as ([]&?);
+      iApply (Count_Typed_Heap.mapsto_valid_generic with "[Hp] Hheap"); try iFrame;
+        eauto with lia.
+  Qed.
+
+
+  Lemma data_op_refinement {T1 T2} j K `{LanguageCtx _ _ T2 Mail.l K} (op: Data.Op T1) E σ:
+    nclose sourceN ⊆ E →
+    {{{ j ⤇ K (Call (DataOp op)) ∗ Registered ∗ source_ctx ∗ source_state σ ∗ HeapInv σ }}}
+      Call (GoLayer.DataOp op) @ E
+    {{{ v, RET v; ∃ h, j ⤇ K (Ret v) ∗ Registered ∗ source_state (RecordSet.set heap (λ _, h) σ)
+                             ∗ HeapInv (RecordSet.set heap (λ _, h) σ)}}}.
+  Proof.
+    iIntros (HE Φ) "(Hj&Hreg&#Hsource&Hstate&Hheap) HΦ".
+    iMod (is_opened_step_inv with "[$] [$] [$]") as (Hopen) "(Hj&Hstate)"; auto.
+    { simpl; auto. }
+    rewrite -wp_fupd.
+    destruct op.
+    - iApply (wp_newAlloc with "[//]").
+      iIntros (p) "!> Hp".
+      iDestruct (HeapInv_non_alloc_inv _ _ 0 with "[$] Hp") as %?; first auto.
+      iMod (ghost_step_call _ _ _ p ((RecordSet.set heap _ σ : l.(OpState)))
+            with "Hj Hsource Hstate") as "(Hj&Hstate&_)".
+      { intros. econstructor. eexists; split; last by econstructor.
+        econstructor; eauto. eapply opened_step; auto. econstructor.
+        * do 2 eexists. split.
+          ** econstructor; eauto.
+          ** do 2 eexists. split; last econstructor.
+             econstructor.
+        * eauto.
+      }
+      { solve_ndisj. }
+      iModIntro. iApply "HΦ". iExists _. iFrame.
+      {
+        rewrite /HeapInv//=.
+        rewrite big_sepDM_updDyn; try intuition.
+        iFrame. simpl. iDestruct "Hp" as "(?&$)"; eauto.
+      }
+    - iMod (deref_step_inv_do with "Hj Hsource Hstate") as (s alloc v Heq) "(Hj&Hstate)".
+      { solve_ndisj. }
+      destruct Heq as (Heq1&Heq2&Heq3).
+      iDestruct (big_sepDM_lookup_acc with "Hheap") as "((Hp&%)&Hheap)".
+      { eauto. }
+      destruct s; try (simpl in Heq2; congruence); simpl.
+      * iApply (wp_ptrDeref' with "Hp").
+        { eauto. }
+        { eauto. }
+        iIntros "!> Hp".
+        iApply "HΦ".
+        iExists (σ.(heap)). iFrame. simpl.
+        destruct σ. iFrame "Hstate".
+        iApply "Hheap". by iFrame.
+      * iApply (wp_ptrDeref' with "Hp").
+        { eauto. }
+        { eauto. }
+        iIntros "!> Hp".
+        iApply "HΦ".
+        iExists (σ.(heap)). iFrame. simpl.
+        destruct σ. iFrame "Hstate".
+        iApply "Hheap". by iFrame.
+    - destruct na; last first.
+      * iMod (store_start_step_inv_do j K with "Hj Hsource Hstate") as (s alloc Heq) "(Hj&Hstate)".
+        { solve_ndisj. }
+        destruct Heq as (Heq1&Heq2).
+        iDestruct (big_sepDM_insert_acc with "Hheap") as "((Hp&%)&Hheap)".
+        { eauto. }
+        destruct s; try (simpl in Heq2; congruence); simpl; [].
+        iApply (wp_ptrStore_start with "Hp").
+        iIntros "!> Hp".
+        iApply "HΦ".
+        iExists _. iFrame.
+        iApply "Hheap". by iFrame.
+      * iMod (store_finish_step_inv_do j K with "Hj Hsource Hstate")
+          as (s alloc alloc' Heq) "(Hj&Hstate)".
+        { solve_ndisj. }
+        destruct Heq as (Heq1&Heq2&Heq3).
+        iDestruct (big_sepDM_insert_acc with "Hheap") as "((Hp&%)&Hheap)".
+        { eauto. }
+        destruct s; try (simpl in Heq3; congruence); simpl; [].
+        destruct args.
+        iApply (wp_ptrStore_finish with "Hp").
+        { eauto. }
+        iIntros "!> Hp".
+        iApply "HΦ".
+        iExists _. iFrame.
+        iApply "Hheap". by iFrame.
+    -
+  Admitted.
+
+End refinement_heap_triples.
